Hoare logic

While.thy
@@ -6,7 +6,7 @@ text {* We define a simple while programming language based on relations *}
 
 text {* 
   Programs are modelled as relations using a standard while programming language:
-  S ::= abort | skip | basic f | S; S' | if b then S else S' fi | while b do S od,
+  S ::= abort | skip | \<langle>f\<rangle> | \<lceil>g\<rceil> | S; S' | if b then S else S' fi | while b do S od,
   where f is a state transformer
 *}
 
@@ -16,33 +16,41 @@ definition abort :: "'s rel" ("abort") where "abort \<equiv> {}"
 
 definition skip :: "'s rel" ("skip") where "skip \<equiv> Id" 
 
-definition torel :: "('s \<Rightarrow> 's) \<Rightarrow> 's rel" ("\<langle>_\<rangle>" 100) where
+definition to_rel :: "('s \<Rightarrow> 's) \<Rightarrow> 's rel" ("\<langle>_\<rangle>" 100) where
   "\<langle>f\<rangle> \<equiv> {(s, f s) | s. True}"
 
 definition seq :: "'s rel \<Rightarrow> 's rel \<Rightarrow> 's rel" (infixr ";" 60) where
   "seq \<equiv> relcomp"
 
 definition cond :: "'s set \<Rightarrow> 's rel \<Rightarrow> 's rel \<Rightarrow> 's rel" where
-  "cond p x y \<equiv> (\<lfloor>p\<rfloor>;x) \<union> (\<lfloor>-p\<rfloor>;y)"
+  "cond b x y \<equiv> (\<lfloor>b\<rfloor>;x) \<union> (\<lfloor>-b\<rfloor>;y)"
 
 definition while :: "'s set \<Rightarrow> 's rel \<Rightarrow> 's rel" where
-  "while p x \<equiv> (\<lfloor>p\<rfloor>;x)\<^sup>*; \<lfloor>-p\<rfloor>"
+  "while b x \<equiv> (\<lfloor>b\<rfloor>;x)\<^sup>*; \<lfloor>-b\<rfloor>"
 
-definition block :: "('s \<Rightarrow> 's) \<Rightarrow> 's rel \<Rightarrow> 's rel" where
-  "block f x \<equiv> \<langle>f\<rangle>; x"
-
+definition dyn :: "('s \<Rightarrow> 's rel) \<Rightarrow> 's rel" ("\<lceil>_\<rceil>" 100) where
+  "\<lceil>g\<rceil> \<equiv> {(s, s'). (s, s') \<in> g s}"
+  
+definition block :: "('s \<Rightarrow> 's) \<Rightarrow> 's rel \<Rightarrow> ('s \<Rightarrow> 's \<Rightarrow> 's) \<Rightarrow> ('s \<Rightarrow> 's \<Rightarrow> 's rel) \<Rightarrow> 's rel" where
+  "block init x ret c \<equiv> \<lceil>\<lambda>s. \<langle>init\<rangle>; x; \<lceil>\<lambda>t. \<langle>ret s\<rangle>; c s t\<rceil> \<rceil>"
+  
 text {* Annotated programs for automatic verification *}
 
-definition awhile :: "('b \<Rightarrow> 's set) \<Rightarrow> 's set \<Rightarrow> 's rel \<Rightarrow> 's rel" where
-  "awhile i p x \<equiv> while p x"
+definition awhile :: "('v \<Rightarrow> 's set) \<Rightarrow> 's set \<Rightarrow> 's rel \<Rightarrow> 's rel" where
+  "awhile i b x \<equiv> while b x"
 
-definition apre :: "('b \<Rightarrow> 's set) \<Rightarrow> 's rel \<Rightarrow> 's rel" where
+definition apre :: "('v \<Rightarrow> 's set) \<Rightarrow> 's rel \<Rightarrow> 's rel" where
   "apre p x \<equiv> x"
 
-definition apost :: "'s rel \<Rightarrow> ('b \<Rightarrow> 's set) \<Rightarrow> 's rel" where
+definition apost :: "'s rel \<Rightarrow> ('v \<Rightarrow> 's set) \<Rightarrow> 's rel" where
   "apost x q \<equiv> x; apre q skip"
 
-definition aprog :: "('b \<Rightarrow> 's set) \<Rightarrow> 's rel \<Rightarrow> ('b \<Rightarrow> 's set) \<Rightarrow> 's rel" where
+definition aprog :: "('v \<Rightarrow> 's set) \<Rightarrow> 's rel \<Rightarrow> ('v \<Rightarrow> 's set) \<Rightarrow> 's rel" where
   "aprog p x q \<equiv> x"
+
+text {* Lift tests to assertions *}
+
+definition assert :: "'a set \<Rightarrow> 'v \<Rightarrow> 'a set" ("<_>") where
+  "<b> \<equiv> \<lambda>_. b"
 
 end
