Syntax.thy
@@ -1,0 +1,46 @@
+theory Syntax
+  imports Hoare
+begin
+
+(* Syntax of the While language *)
+
+syntax
+  "_quote" :: "'b \<Rightarrow> ('a \<Rightarrow> 'b)" ("(\<guillemotleft>_\<guillemotright>)" [0] 1000)
+  "_antiquote" :: "('a \<Rightarrow> 'b) \<Rightarrow> 'a" ("`_" [1000] 1000) 
+  "_subst" :: "'a set \<Rightarrow> 'b \<Rightarrow> idt \<Rightarrow> 'a set" ("_[_'/`_]" [1000] 999)
+  "_assign" :: "idt \<Rightarrow> 'b \<Rightarrow> 'a rel" ("(`_ :=/ _)" [0, 65] 62)
+  "_cond" :: "'a set \<Rightarrow> 'a rel \<Rightarrow> 'a rel \<Rightarrow> 'a rel" ("(0if _ then//  _//else//  _//fi)" [0,0,0] 62)
+  "_cond_skip" :: "'a set \<Rightarrow> 'a rel \<Rightarrow> 'a rel" ("(0if _//then _//fi)" [0,0] 62)
+  "_while" :: "'a set \<Rightarrow> 'a rel \<Rightarrow> 'a rel" ("(0while  _//do  _//od)" [0, 0] 62)
+  "_awhile" :: "'a set \<Rightarrow> 'a set \<Rightarrow> 'a rel \<Rightarrow> 'a rel" ("(0while _//inv  _//do _//od)" [0, 0, 0] 62)
+
+ML {*
+fun quote_tr [t] = Syntax_Trans.quote_tr @{syntax_const "_antiquote"} t
+    | quote_tr ts = raise TERM ("quote_tr", ts)
+*}
+
+parse_translation {*
+  [(@{syntax_const "_quote"}, K quote_tr)]
+*}
+
+translations
+  "p [t/`u]" == "CONST Collect \<guillemotleft> `(_update_name u (\<lambda>_. t)) \<in> p \<guillemotright>"
+  "`u := t" => "CONST to_rel \<guillemotleft>`(_update_name u (\<lambda>_. t))\<guillemotright>"
+  "if b then x else y fi" => "CONST cond (CONST Collect \<guillemotleft>b\<guillemotright>) x y"
+  "if b then x fi" == "if b then x else skip fi"
+  "while b inv i do x od" => "CONST awhile (CONST Collect \<guillemotleft>i\<guillemotright>) (CONST Collect \<guillemotleft>b\<guillemotright>) x"
+  
+  
+(* Syntax of Hoare logic *)
+
+syntax
+  "_ht" :: "'a set \<Rightarrow> 'a rel \<Rightarrow> 'a set \<Rightarrow> bool" ("\<turnstile> \<lbrace> _ \<rbrace>// _// \<lbrace> _ \<rbrace>" [0, 55, 0] 50)
+translations
+  "\<turnstile> \<lbrace> p \<rbrace> x \<lbrace> q \<rbrace>" == "CONST ht (%_. CONST Collect \<guillemotleft>p\<guillemotright>) x (%_. CONST Collect \<guillemotleft>q\<guillemotright>)"
+  
+record test = 
+  i :: nat
+  j :: nat
+  
+lemma "\<turnstile> \<lbrace> True \<rbrace> block (\<lambda>s. s\<lparr>i := j s\<rparr>) {} (\<lambda>s t. t\<lparr> i := i s\<rparr>) (\<lambda>s t. skip) \<lbrace> True \<rbrace>"
+end
